prove soundness of theta d

Clean/Gadgets/Keccak/ThetaD.lean
@@ -8,16 +8,16 @@ namespace Gadgets.Keccak.ThetaD
 variable {p : ℕ} [Fact p.Prime]
 variable [p_large_enough: Fact (p > 512)]
 
-open Provable (field field2 fields)
 open FieldUtils (mod_256 floordiv)
 open Xor (xor_u64)
 open Clean.Gadgets.Keccak256
+open Gadgets.Rotation64.Theorems (rot_right64)
 
 @[reducible]
-def Inputs := vec_provable U64 5
+def Inputs := ProvableVector U64 5
 
 @[reducible]
-def Outputs := vec_provable U64 5
+def Outputs := ProvableVector U64 5
 
 def theta_d (state : Var Inputs (F p)) : Circuit (F p) (Var Outputs (F p)) := do
   let c0 ← subcircuit (Gadgets.Rotation64.circuit 1) (state.get 1)
@@ -37,22 +37,102 @@ def theta_d (state : Var Inputs (F p)) : Circuit (F p) (Var Outputs (F p)) := do
 
   return #v[c0, c1, c2, c3, c4]
 
+instance elaborated : ElaboratedCircuit (F p) Inputs (Var Outputs (F p)) where
+  main := theta_d
+  local_length _ := 160
+  output _ i0 := #v[
+    var_from_offset U64 (i0 + 24),
+    var_from_offset U64 (i0 + 56),
+    var_from_offset U64 (i0 + 88),
+    var_from_offset U64 (i0 + 120),
+    var_from_offset U64 (i0 + 152)
+  ]
+
 def assumptions (state : Inputs (F p)) : Prop :=
-  -- TODO
-  true
+  ∀ i : Fin 5, state[i].is_normalized
 
 def spec (state : Inputs (F p)) (out: Outputs (F p)) : Prop :=
-  true
+  let h_norm := out[0].is_normalized ∧ out[1].is_normalized ∧
+            out[2].is_normalized ∧ out[3].is_normalized ∧ out[4].is_normalized
 
-def circuit : FormalCircuit (F p) Inputs Outputs where
-  main := theta_d
-  assumptions := assumptions
-  spec := spec
-  local_length _ := sorry
-  local_length_eq := sorry
-  output _ i0 := sorry
-  output_eq := sorry
+  let h0 := out[0].value = (rot_right64 (state[1].value) 1 |>.xor state[4].value)
+  let h1 := out[1].value = (rot_right64 (state[2].value) 1 |>.xor state[0].value)
+  let h2 := out[2].value = (rot_right64 (state[3].value) 1 |>.xor state[1].value)
+  let h3 := out[3].value = (rot_right64 (state[4].value) 1 |>.xor state[2].value)
+  let h4 := out[4].value = (rot_right64 (state[0].value) 1 |>.xor state[3].value)
 
-  soundness := by sorry
-  completeness := by sorry
+  h_norm ∧ h0 ∧ h1 ∧ h2 ∧ h3 ∧ h4
+
+theorem soundness : Soundness (F p) assumptions spec := by
+  intro i0 env state_var state h_input state_norm h_holds
+  simp only [circuit_norm] at h_input
+  dsimp only [assumptions] at state_norm
+  dsimp only [circuit_norm, theta_d, Xor.circuit, Rotation64.circuit] at h_holds
+  simp only [circuit_norm, subcircuit_norm] at h_holds
+  dsimp only [Xor.assumptions, Xor.spec, Rotation64.assumptions, Rotation64.spec] at h_holds
+  simp [add_assoc, and_assoc] at h_holds
+
+  have u64_from_offset (i : ℕ) : var_from_offset (F:=(F p)) U64 (i0 + i) = ⟨var ⟨i0 + i⟩, var ⟨i0 + i + 1⟩, var ⟨i0 + i + 2⟩, var ⟨i0 + i + 3⟩, var ⟨i0 + i + 4⟩, var ⟨i0 + i + 5⟩, var ⟨i0 + i + 6⟩, var ⟨i0 + i + 7⟩⟩ := by
+    simp only [var_from_offset, from_vars, from_elements, Vector.natInit, add_zero, Vector.push_mk,
+      Nat.reduceAdd, List.push_toArray, List.nil_append, List.cons_append]
+
+  rw [←u64_from_offset 16, ←u64_from_offset 48, ←u64_from_offset 80, ←u64_from_offset 112, ←u64_from_offset 144] at h_holds
+  clear u64_from_offset
+
+  have s0 : eval env (state_var[0]) = state[0] := by rw [←h_input, Vector.getElem_map]
+  have s1 : eval env (state_var[1]) = state[1] := by rw [←h_input, Vector.getElem_map]
+  have s2 : eval env (state_var[2]) = state[2] := by rw [←h_input, Vector.getElem_map]
+  have s3 : eval env (state_var[@Fin.val 5 3]) = state[3] := by rw [←h_input, Vector.getElem_map]; rfl
+  have s4 : eval env (state_var[@Fin.val 5 4]) = state[4] := by rw [←h_input, Vector.getElem_map]; rfl
+
+  rw [s0, s1, s2, s3, s4] at h_holds
+  clear s0 s1 s2 s3 s4
+
+  simp [circuit_norm, spec]
+
+  -- lift everything to U64 variables
+  set c0 := eval env <| var_from_offset (F:=(F p)) U64 (i0 + 16)
+  set c0' := eval env <| var_from_offset (F:=(F p)) U64 (i0 + 24)
+  set c1 := eval env <| var_from_offset (F:=(F p)) U64 (i0 + 48)
+  set c1' := eval env <| var_from_offset (F:=(F p)) U64 (i0 + 56)
+  set c2 := eval env <| var_from_offset (F:=(F p)) U64 (i0 + 80)
+  set c2' := eval env <| var_from_offset (F:=(F p)) U64 (i0 + 88)
+  set c3 := eval env <| var_from_offset (F:=(F p)) U64 (i0 + 112)
+  set c3' := eval env <| var_from_offset (F:=(F p)) U64 (i0 + 120)
+  set c4 := eval env <| var_from_offset (F:=(F p)) U64 (i0 + 144)
+  set c4' := eval env <| var_from_offset (F:=(F p)) U64 (i0 + 152)
+
+  obtain ⟨ h_rot0, h_xor0, h_rot1, h_xor1, h_rot2, h_xor2, h_rot3, h_xor3, h_rot4, h_xor4 ⟩ := h_holds
+
+  specialize h_rot0 (state_norm 1)
+  specialize h_xor0 h_rot0.right (state_norm 4)
+  specialize h_rot1 (state_norm 2)
+  specialize h_xor1 h_rot1.right (state_norm 0)
+  specialize h_rot2 (state_norm 3)
+  specialize h_xor2 h_rot2.right (state_norm 1)
+  specialize h_rot3 (state_norm 4)
+  specialize h_xor3 h_rot3.right (state_norm 2)
+  specialize h_rot4 (state_norm 0)
+  specialize h_xor4 h_rot4.right (state_norm 3)
+
+  simp [h_xor0, h_xor1, h_xor2, h_xor3, h_xor4, h_rot0, h_rot1, h_rot2, h_rot3, h_rot4]
+
+
+theorem completeness : Completeness (F p) Outputs assumptions := by
+  intro i0 env state_var h_env state h_input h_assumptions
+  simp only [circuit_norm] at h_input
+  dsimp only [circuit_norm, theta_d, Xor.circuit, Rotation64.circuit]
+  simp only [circuit_norm, subcircuit_norm]
+  dsimp only [Xor.assumptions, Xor.spec]
+  simp [add_assoc]
+  sorry
+
+def circuit : FormalCircuit (F p) Inputs Outputs := {
+  elaborated with
+  assumptions
+  spec
+  soundness
+  completeness
+}
+
 end Gadgets.Keccak.ThetaD
